Rename include_defs && Tweak unsound definition

compose/Skeleton.v
@@ -251,6 +251,31 @@ I think "sim_skenv_monotone" should be sufficient.
 
   Definition empty: t := @Genv.empty_genv _ _ [].
 
+  (* Note:
+       1) It is more natural to define this predicate in `Genv` namespace, not `AST` namespace. (because of dependency)
+       2) Natural ordering of parameters is __name__: Genv.t -> program -> Prop. (`ge.(__name__) prog`)
+
+       Note: why not just name it `incl`?
+       It is confusing as `List.incl` has an opposite direction.
+       I think `List.incl` is abbreviation of `List.is_included`.
+       le a b        === a.(le) b        === a <= b
+       List.incl a b === a.(List.incl) b === a <= b
+       includes a b  === a.(includes) b  === a >= b
+   *)
+
+  (* TODO: Can we forward-reference Sk.t ? *)
+  Inductive includes (skenv: SkEnv.t) (sk: AST.program (AST.fundef signature) unit): Prop :=
+  | includes_intro
+      (DEFS: forall
+          id gd0
+          (DEF: sk.(prog_defmap) ! id = Some gd0)
+        ,
+          exists blk gd1, (<<SYMB: skenv.(Genv.find_symbol) id = Some blk>>) /\
+                          (<<DEF: skenv.(Genv.find_def) blk = Some gd1>>) /\
+                          (<<MATCH: linkorder gd0 gd1>>))
+      (PUBS: incl sk.(prog_public) skenv.(Genv.genv_public))
+  .
+
 End SkEnv.
 
 Hint Unfold SkEnv.empty.
@@ -440,29 +465,6 @@ End Sk.
 
 Hint Unfold skdef_of_gdef skdefs_of_gdefs Sk.load_skenv Sk.load_mem Sk.empty.
 
-Lemma include_defs_lift
-      F V get_sg
-      (prog: AST.program (AST.fundef F) V) skenv_link
-      (INCL: include_defs eq (Sk.of_program get_sg prog) skenv_link)
-  :
-    <<INCL: include_defs
-              (fun fdef skdef => skdef_of_gdef get_sg fdef = skdef) prog skenv_link>>
-.
-Proof.
-  {
-    ii. exploit (INCL id (skdef_of_gdef get_sg def0)).
-    - clear - DEF.
-      unfold prog_defmap in *. destruct prog. ss.
-      exploit (PTree_Properties.of_list_related (fun e1 e2 => @skdef_of_gdef _ V get_sg e1 = e2)); cycle 1.
-      { i. inv H; rewrite DEF in *; clarify. rewrite <- H1. ss. }
-      {
-        eapply list_forall2_imply.
-        - eapply list_forall2_map.
-        - i. ss. clarify.
-      }
-    - i. des. esplits; eauto.
-  }
-Qed.
 
 
 
