backend/DeadcodeproofC.v
@@ -23,7 +23,8 @@ Variable skenv_link_src skenv_link_tgt: SkEnv.t.
 Variable sm_link: SimMem.t.
 Hypothesis (SIMSKENVLINK: exists ss_link, SimSymb.sim_skenv sm_link ss_link skenv_link_src skenv_link_tgt).
 Variables prog tprog: program.
-Hypothesis INCL: include_defs eq (Sk.of_program fn_sig prog) skenv_link_src.
+Hypothesis INCLSRC: SkEnv.includes skenv_link_src (Sk.of_program fn_sig prog).
+Hypothesis INCLTGT: SkEnv.includes skenv_link_src (Sk.of_program fn_sig prog).
 
 Hypothesis TRANSL: match_prog prog tprog.
 Let ge := (SkEnv.revive (SkEnv.project skenv_link_src (defs prog)) prog).
