common/GlobalenvsC.v
@@ -51,17 +51,8 @@ Ltac align_opt :=
 
 
 
-Section INCLUDEDEFS.
 
-Context {A B V W: Type} (R: globdef A V -> globdef B W -> Prop).
 
-Definition include_defs (p: AST.program A V) (ge: Genv.t B W) : Prop :=
-  forall id def0 (DEF: p.(prog_defmap) ! id = Some def0),
-  exists blk def1, (<<SYMB: ge.(Genv.find_symbol) id = Some blk>>) /\
-                   (<<DEF: ge.(Genv.find_def) blk = Some def1>>) /\
-                   (<<MATCH: R def0 def1>>).
-
-End INCLUDEDEFS.
 
 Section EXTERNAL.
 
