proof/SimMod.v
@@ -69,10 +69,11 @@ Context `{SM: SimMem.class} {SS: SimSymb.class SM} {SU: Sound.class}.
       (* ) *)
       (SIMMS: forall
           skenv_link_src skenv_link_tgt
+          (INCLSRC: SkEnv.includes skenv_link_src mp.(src).(Mod.sk))
+          (INCLTGT: SkEnv.includes skenv_link_tgt mp.(tgt).(Mod.sk))
           ss_link
           (SSLE: SimSymb.le mp.(ss) mp.(src) mp.(tgt) ss_link)
           sm_init_link
-          (INCLUDE: include_defs eq mp.(src).(Mod.sk) skenv_link_src)
           (SIMSKENVLINK: SimSymb.sim_skenv sm_init_link ss_link skenv_link_src skenv_link_tgt)
         ,
           <<SIMMSP: ModSemPair.sim mp.(to_msp skenv_link_src skenv_link_tgt sm_init_link)>>)
